src/Pipit.Exp.Causality.fst
@@ -3,13 +3,14 @@ module Pipit.Exp.Causality
 
 open Pipit.Exp.Base
 open Pipit.Exp.Binding
-// open Pipit.Exp.Bigstep
+open Pipit.Exp.Binding.Properties
+open Pipit.Exp.Bigstep
 
 module C = Pipit.Context
 
-(* Causality: does expression `e` have a dependency on the most-recent value of expression `e'`?
+(* Direct dependencies: does expression `e` have a non-delayed dependency on bound-variable `i`?
     *)
-let rec direct_dependency (e: exp 'c 'a) (i: C.index { C.has_index 'c i }) : Tot bool (decreases e) =
+let rec direct_dependency (e: exp 'c 'a) (i: C.index) : Tot bool (decreases e) =
   match e with
   | XVal _ -> false
   | XVar _ -> false
@@ -21,10 +22,15 @@ let rec direct_dependency (e: exp 'c 'a) (i: C.index { C.has_index 'c i }) : Tot
   | XLet b e1 e2 -> direct_dependency e1 i || direct_dependency e2 (i + 1)
   | XCheck name e1 e2 -> direct_dependency e1 i || direct_dependency e2 i
 
+(* Causality: are all references to recursive streams delayed?
+   All causal expressions make progress.
+   We also sneak in a well-formedness check here that there are no free
+   variables. This is really a different check, but it's convenient.
+*)
 let rec causal (e: exp 'c 'a): Tot bool (decreases e) =
   match e with
   | XVal _ -> true
-  | XVar _ -> true
+  | XVar _ -> false // no free variables
   | XBVar _ -> true
   | XApp e1 e2 -> causal e1 && causal e2
   | XFby _ e1 -> causal e1
@@ -33,261 +39,363 @@ let rec causal (e: exp 'c 'a): Tot bool (decreases e) =
   | XLet b e1 e2 -> causal e1 && causal e2
   | XCheck _ e1 e2 -> causal e1 && causal e2
 
-let rec direct_dependency_lift (e: exp 'c 'a) (i: C.index { C.has_index 'c i }) (i': C.index { i' <= List.Tot.length 'c }) (t: Type):
-    Lemma (ensures direct_dependency e i == direct_dependency (lift1' e i' t) (i + 1)) (decreases e) =
-  admit ()
+#push-options "--split_queries always"
 
-  // match e with
-  // | XVal _ -> ()
-  // | XVar _ -> ()
-  // | XPrim2 p e1 e2 ->
-  //   direct_dependency_lift e1 e' x;
-  //   direct_dependency_lift e2 e' x
-  // | XIte ep e1 e2 ->
-  //   direct_dependency_lift ep e' x;
-  //   direct_dependency_lift e1 e' x;
-  //   direct_dependency_lift e2 e' x
-  // | XPre _ -> ()
-  // | XThen e1 e2 ->
-  //   direct_dependency_lift e1 e' x;
-  //   direct_dependency_lift e2 e' x
-  // | XMu e1 ->
-  //   direct_dependency_lift e1 (lift e' 0) (x + 1);
-  //   lift_lift_commute e' x 0
-  // | XLet e1 e2 ->
-  //   direct_dependency_lift e1 e' x;
-  //   direct_dependency_lift e2 (lift e' 0) (x + 1);
-  //   lift_lift_commute e' x 0
-
-let rec direct_dependency_not_subst (i: C.index { C.has_index 'c i }) (i': C.index { i' < i })
-  (e: exp 'c 'a { ~ (direct_dependency e i) })
-  (p: exp (C.drop1 'c i') (C.get_index 'c i') { ~ (direct_dependency p (i - 1)) }):
-    Lemma (ensures ~ (direct_dependency (subst1' e i' p) (i - 1))) (decreases e) =
-  admit ()
-  // match e with
-  // | XVal _ -> ()
-  // | XVar x'' -> ()
-  // | XPrim2 prim e1 e2 ->
-  //   direct_dependency_not_subst x x' e1 p;
-  //   direct_dependency_not_subst x x' e2 p
-  // | XIte ep e1 e2 ->
-  //   direct_dependency_not_subst x x' ep p;
-  //   direct_dependency_not_subst x x' e1 p;
-  //   direct_dependency_not_subst x x' e2 p
-  // | XPre _ -> ()
-  // | XThen e1 e2 ->
-  //   direct_dependency_not_subst x x' e1 p;
-  //   direct_dependency_not_subst x x' e2 p
-  // | XMu e1 ->
-  //   direct_dependency_lift p (XVar (x - 1)) 0;
-  //   direct_dependency_not_subst (x + 1) (x' + 1) e1 (lift p 0)
-  // | XLet e1 e2 ->
-  //   direct_dependency_lift p (XVar (x - 1)) 0;
-  //   direct_dependency_not_subst x x' e1 p;
-  //   direct_dependency_not_subst (x + 1) (x' + 1) e2 (lift p 0)
-
-(* Shelve: proofs about causality, will need to be restated on single-element semantics *)
-
-let rec direct_dependency_not_subst2 (x: var) (x': var { x < x' }) (e p: exp):
-    Lemma
-      (requires not (direct_dependency (subst e x' p) (XVar x)))
-      (ensures not (direct_dependency e (XVar x))) (decreases e) =
+(* used by lemma_causal_lift *)
+let rec lemma_direct_dependency_lift (e: exp 'c 'a) (i: C.index { C.has_index 'c i }) (i': C.index { i < i' /\ i' <= List.Tot.length 'c }) (t: Type):
+    Lemma (ensures direct_dependency e i == direct_dependency (lift1' e i' t) i) (decreases e) =
   match e with
-  | XVal _ -> ()
-  | XVar x'' -> ()
-  | XPrim2 prim e1 e2 ->
-    direct_dependency_not_subst2 x x' e1 p;
-    direct_dependency_not_subst2 x x' e2 p
-  | XPre _ -> ()
-  | XThen e1 e2 ->
-    direct_dependency_not_subst2 x x' e1 p;
-    direct_dependency_not_subst2 x x' e2 p
-  | XMu e1 ->
-    direct_dependency_lift p (XVar x') 0;
-    direct_dependency_not_subst2 (x + 1) (x' + 1) e1 (lift p 0)
-  | XLet e1 e2 ->
-    direct_dependency_not_subst2 x x' e1 p;
-    direct_dependency_not_subst2 (x + 1) (x' + 1) e2 (lift p 0)
+  | XVal _ | XVar _ | XBVar _ -> ()
+  | XMu _ e1 ->
+    lemma_direct_dependency_lift e1 (i + 1) (i' + 1) t
 
-
-let rec bigstep_no_dep_no_difference (#outer #inner1 #inner2: nat) (e: exp { ~ (direct_dependency e (XVar inner1)) })
-  (streams1: C.table (outer + 1) inner1)
-  (streams2: C.table (outer + 1) inner2)
-  (row: C.vector value outer) (v v': value)
-  (vs: C.vector value (outer + 1))
-  (hBS: bigstep
-    (C.table_map_append streams1 (C.table_map_append (C.table_of_values (v :: row)) streams2))
-    e
-    vs):
-  Tot (bigstep
-        (C.table_map_append streams1 (C.table_map_append (C.table_of_values (v' :: row)) streams2))
-        e vs) (decreases hBS) =
-  let tv  = C.table_of_values (v :: row) in
-  let tv' = C.table_of_values (v' :: row) in
-  let t2  = C.table_map_append tv streams2 in
-  let t2' = C.table_map_append tv' streams2 in
-  let t  = C.table_map_append streams1 t2 in
-  let t' = C.table_map_append streams1 t2' in
-  match hBS with
-  | BSVal _ v ->
-    C.table_const_const t t' v;
-    BSVal _ v
-  | BSVar _ x ->
-    assert (x <> inner1);
-    if x < inner1
-    then
-    begin
-        C.table_index_append_inner1 streams1 t2 x;
-        C.table_index_append_inner1 streams1 t2' x;
-        BSVar _ x
-    end
-    else
-    begin
-        C.table_index_append_inner2 streams1 t2 x;
-        C.table_index_append_inner2 tv streams2 (x - inner1);
-        C.table_index_append_inner2 streams1 t2' x;
-        C.table_index_append_inner2 tv' streams2 (x - inner1);
-        BSVar _ x
-    end
-  | BSPrim2 _ p e1 e2 vs1 vs2 hBS1 hBS2 ->
-    let hBS1' = bigstep_no_dep_no_difference e1 streams1 streams2 row v v' vs1 hBS1 in
-    let hBS2' = bigstep_no_dep_no_difference e2 streams1 streams2 row v v' vs2 hBS2 in
-    BSPrim2 _ p e1 e2 vs1 vs2 hBS1' hBS2'
-  | BSPre s0 ss e1 vs1 hBS1 ->
-    let s0' = C.table_hd t' in
-    BSPre s0' ss e1 vs1 hBS1
-  | BSThen _ e1 e2 vs1 vs2 hBS1 hBS2 ->
-    let hBS1' = bigstep_no_dep_no_difference e1 streams1 streams2 row v v' vs1 hBS1 in
-    let hBS2' = bigstep_no_dep_no_difference e2 streams1 streams2 row v v' vs2 hBS2 in
-    BSThen _ e1 e2 vs1 vs2 hBS1' hBS2'
-  | BSMu _ e1 vs1 hBS1 ->
-    let e1' = subst e1 0 (XMu e1) in
-    direct_dependency_not_subst (inner1 + 1) 0 e1 (XMu e1);
-    let hBS1' = bigstep_no_dep_no_difference e1' streams1 streams2 row v v' vs1 hBS1 in
-    BSMu _ e1 vs1 hBS1'
-  | BSLet _ e1 e2 vs2 hBS2 ->
-    let e1' = subst e2 0 e1 in
-    direct_dependency_not_subst (inner1 + 1) 0 e2 e1;
-    let hBS2' = bigstep_no_dep_no_difference e1' streams1 streams2 row v v' vs2 hBS2 in
-    BSLet _ e1 e2 vs2 hBS2'
-
-
-(* I originally thought that something like the following should hold:
-   if e evaluates to a value, then e is causal
-   but this doesn't work for empty input streams, and also doesn't work for
-   recursive binders that are nested arbitrarily inside pre combinators, eg
-   > pre (pre (pre (pre (mu x. x))))
-
-*)
-// let rec bigstep_means_causal (#outer #inner: nat) (e: exp)
-//   (streams: C.table outer inner)
-//   (vs: C.vector value outer)
-//   (hBS: bigstep streams e vs):
-//     Lemma (ensures causal e) (decreases hBS) =
-//
-
-// XXX: cannot state this on direct_dependency with var...
-// but can state:
-let rec direct_dep_XVar__direct_dep_subst (e e': exp) (x: var):
-  Lemma (requires direct_dependency e x /\ direct_dependency e' x')
-        (ensures direct_dependency (subst e x e') x') =
-  admit ()
-//
-// let rec direct_dep_XVar__direct_dep_subst (e e': exp) (x: var):
-//   Lemma (requires direct_dependency e (XVar x))
-//         (ensures direct_dependency (subst e x e') e') =
-//   match e with
-//   | XPrim2 _ e1 e2 ->
-//     if direct_dependency e1 (XVar x)
-//     then direct_dep_XVar__direct_dep_subst e1 e' x
-//     else direct_dep_XVar__direct_dep_subst e2 e' x
-//   | XMu e1 ->
-//     direct_dep_XVar__direct_dep_subst e1 (lift e' 0) (x + 1)
-//   | XThen e1 e2 ->
-//     if direct_dependency e1 (XVar x)
-//     then direct_dep_XVar__direct_dep_subst e1 e' x
-//     else direct_dep_XVar__direct_dep_subst e2 e' x
-//   | XLet e1 e2 ->
-//     if direct_dependency e1 (XVar x)
-//     then direct_dep_XVar__direct_dep_subst e1 e' x
-//     else direct_dep_XVar__direct_dep_subst e2 (lift e' 0) (x + 1)
-//   | _ -> ()
-
-let causal_subst__causal_XMu (e: exp) (n: nat):
-  Lemma (requires causal (XMu e))
-        (ensures causal (subst e 0 (XMu e))) =
-  assert (not (direct_dependency e (XVar 0)));
-  admit ()
-
-
-let bigstep_recursive_XMu (#outer #inner: nat) (e: exp)
-  (streams: C.table (outer + 1) inner)
-  (vs: C.vector value outer) (v v': value)
-  (hBSmu: bigstep streams (XMu e) (v :: vs)):
-    bigstep (C.table_map_append (C.table_of_values (v' :: vs)) streams) e (v :: vs) =
-    // bigstep_means_causal_up_to_depth _ _ _ hBSmu;
-    let hBS' = bigstep_substitute_XMu e streams _ hBSmu in
-    C.table_map_append_empty1 (C.table_map_append (C.table_of_values (v :: vs)) streams);
-    C.table_map_append_empty1 (C.table_map_append (C.table_of_values (v' :: vs)) streams);
-    bigstep_no_dep_no_difference e (C.table_empty (outer + 1)) streams vs v v' (v :: vs) hBS'
-
-
-let rec bigstep_empty (inner: nat)
-  (e: exp { causal e /\ wf e inner }):
-    Tot (bigstep #inner (C.Table []) e []) (decreases e) =
-  match e with
-  | XVal v -> BSVal _ v
-  | XVar x -> BSVar _ x
-  | XPre e1 -> BSPre0 e1
-  // TODO bigstep_empty XMu: looks pretty true, but needs stronger induction hypothesis.
-  // TODO bigstep_empty XLet
-  | XMu e1 -> admit ()
   | _ -> admit ()
 
-let rec bigstep_monotone_inv' (#outer #inner: nat)
-  (#streams: C.table (outer + 1) inner) (#e: exp { causal e /\ wf e inner }) (#vs: C.vector value outer)
-  (hBS: bigstep (C.table_tl streams) e vs):
-    Tot (v': value & bigstep streams e (v' :: vs)) (decreases hBS) =
-  match hBS with
-  | BSVal _ v -> (| v, BSVal _ v |)
-  | BSVar _ x -> (| C.row_index (C.table_hd streams) x, BSVar _ x |)
-  | BSPrim2 _ p e1 e2 vs1 vs2 hBS1 hBS2 ->
-    let (| v1', hBS1' |) = bigstep_monotone_inv' hBS1 in
-    let (| v2', hBS2' |) = bigstep_monotone_inv' hBS2 in
-    (| eval_prim2 p v1' v2', BSPrim2 _ p e1 e2 (v1' :: vs1) (v2' :: vs2) hBS1' hBS2' |)
+(* used by lemma_causal_subst *)
+let rec lemma_direct_dependency_not_subst (i: C.index { C.has_index 'c i }) (i': C.index { C.has_index 'c i' /\ i < i' })
+  (e: exp 'c 'a { ~ (direct_dependency e i) /\ ~ (direct_dependency e i') })
+  (p: exp (C.drop1 'c i') (C.get_index 'c i')):
+    Lemma (ensures ~ (direct_dependency (subst1' e i' p) i)) (decreases e) =
+  match e with
+  | XVal _ | XVar _ | XBVar _ -> ()
+  | XMu _ e1 ->
+    lemma_direct_dependency_not_subst (i + 1) (i' + 1) e1 (lift1 p 'a)
+  | _ -> admit ()
 
-  | BSPre r s e1 vs hBS1 ->
-    let (| v1', hBS1' |) = bigstep_monotone_inv' #(outer - 1) #inner #(C.table_append (C.table1 r) s) hBS1 in
-    (| v1', BSPre (C.table_hd streams) (C.table_tl streams) e1 (v1' :: vs) hBS1' |)
+(* used by lemma_bigstep_substitute_intros_no_dep *)
+let rec lemma_direct_dependency_not_subst' (i: C.index { C.has_index 'c i }) (i': C.index { C.has_index 'c i' /\ i' <= i })
+  (e: exp 'c 'a { ~ (direct_dependency e (i + 1)) })
+  (p: exp (C.drop1 'c i') (C.get_index 'c i') { ~ (direct_dependency p i ) }):
+    Lemma (ensures ~ (direct_dependency (subst1' e i' p) i)) (decreases e) =
+  match e with
+  | XVal _ -> ()
+  | XVar _ -> ()
+  | XBVar _ -> ()
+  | XMu _ e1 ->
+    // TODO requires extra lemma lemma_direct_dependency_lift p i 0 'a;
+    assume (~ (direct_dependency (lift1 p 'a) (i + 1)));
+    lemma_direct_dependency_not_subst' (i + 1) (i' + 1) e1 (lift1 p 'a)
+    // admit ()
+  | _ -> admit ()
 
-  | BSPre0 e1 ->
-    let hBS': bigstep (C.Table []) e1 [] = bigstep_empty inner e1 in
-    (| xpre_init, BSPre (C.table_hd streams) (C.Table []) e1 [] hBS' |)
+(* old statements, might be necessary *)
+// let rec direct_dependency_not_subst (i: C.index { C.has_index 'c i }) (i': C.index { i' < i })
+//   (e: exp 'c 'a { ~ (direct_dependency e i) })
+//   (p: exp (C.drop1 'c i') (C.get_index 'c i') { ~ (direct_dependency p (i - 1)) }):
+//     Lemma (ensures ~ (direct_dependency (subst1' e i' p) (i - 1))) (decreases e) =
+// let rec direct_dependency_not_subst2 (i: C.index { C.has_index 'c i }) (i': C.index { C.has_index 'c i' /\ i < i' })
+//   (e: exp 'c 'a)
+//   (p: exp (C.drop1 'c i') (C.get_index 'c i')):
+//     Lemma
+//       (requires ~ (direct_dependency (subst1' e i' p) i))
+//       (ensures ~ (direct_dependency e i)) (decreases e) =
 
-  | BSMu _ e1 vs1 hBS1 ->
-    let e1' = subst e1 0 (XMu e1) in
-    subst_preserves_wf e1 (XMu e1) inner 0;
-    causal_subst__causal_XMu e1 inner;
-    let (| v1', hBS1' |) = bigstep_monotone_inv' hBS1 in
-      (| v1', BSMu _ e1 (v1' :: vs1) hBS1' |)
-  | BSThen _ e1 e2 vs1 vs2 hBS1 hBS2 ->
-    let (| v1', hBS1' |) = bigstep_monotone_inv' hBS1 in
-    let (| v2', hBS2' |) = bigstep_monotone_inv' hBS2 in
-    (| (if outer = 0 then v1' else v2'), BSThen _ e1 e2 (v1' :: vs1) (v2' :: vs2) hBS1' hBS2' |)
-  | BSLet _ _ _ _ _ -> admit ()
+(* used by lemma_bigstep_recursive_XMu *)
+let rec lemma_bigstep_no_dep (e: exp (List.Tot.append 'c ('b :: 'd)) 'a { ~ (direct_dependency e (List.Tot.length 'c)) })
+  (history: list (C.row (List.Tot.append 'c ('b :: 'd))))
+  (rowc: C.row 'c)
+  (rowd: C.row 'd)
+  (b b': 'b)
+  (a: 'a)
+  (hBS: bigstep
+    (C.row_append rowc (C.row_cons b rowd) :: history)
+    e
+    a):
+  Tot (bigstep
+        (C.row_append rowc (C.row_cons b' rowd) :: history)
+        e a) (decreases hBS) =
+  admit ()
+
+  // let tv  = C.table_of_values (v :: row) in
+  // let tv' = C.table_of_values (v' :: row) in
+  // let t2  = C.table_map_append tv streams2 in
+  // let t2' = C.table_map_append tv' streams2 in
+  // let t  = C.table_map_append streams1 t2 in
+  // let t' = C.table_map_append streams1 t2' in
+  // match hBS with
+  // | BSVal _ v ->
+  //   C.table_const_const t t' v;
+  //   BSVal _ v
+  // | BSVar _ x ->
+  //   assert (x <> inner1);
+  //   if x < inner1
+  //   then
+  //   begin
+  //       C.table_index_append_inner1 streams1 t2 x;
+  //       C.table_index_append_inner1 streams1 t2' x;
+  //       BSVar _ x
+  //   end
+  //   else
+  //   begin
+  //       C.table_index_append_inner2 streams1 t2 x;
+  //       C.table_index_append_inner2 tv streams2 (x - inner1);
+  //       C.table_index_append_inner2 streams1 t2' x;
+  //       C.table_index_append_inner2 tv' streams2 (x - inner1);
+  //       BSVar _ x
+  //   end
+  // | BSPrim2 _ p e1 e2 vs1 vs2 hBS1 hBS2 ->
+  //   let hBS1' = bigstep_no_dep_no_difference e1 streams1 streams2 row v v' vs1 hBS1 in
+  //   let hBS2' = bigstep_no_dep_no_difference e2 streams1 streams2 row v v' vs2 hBS2 in
+  //   BSPrim2 _ p e1 e2 vs1 vs2 hBS1' hBS2'
+  // | BSPre s0 ss e1 vs1 hBS1 ->
+  //   let s0' = C.table_hd t' in
+  //   BSPre s0' ss e1 vs1 hBS1
+  // | BSThen _ e1 e2 vs1 vs2 hBS1 hBS2 ->
+  //   let hBS1' = bigstep_no_dep_no_difference e1 streams1 streams2 row v v' vs1 hBS1 in
+  //   let hBS2' = bigstep_no_dep_no_difference e2 streams1 streams2 row v v' vs2 hBS2 in
+  //   BSThen _ e1 e2 vs1 vs2 hBS1' hBS2'
+  // | BSMu _ e1 vs1 hBS1 ->
+  //   let e1' = subst e1 0 (XMu e1) in
+  //   direct_dependency_not_subst (inner1 + 1) 0 e1 (XMu e1);
+  //   let hBS1' = bigstep_no_dep_no_difference e1' streams1 streams2 row v v' vs1 hBS1 in
+  //   BSMu _ e1 vs1 hBS1'
+  // | BSLet _ e1 e2 vs2 hBS2 ->
+  //   let e1' = subst e2 0 e1 in
+  //   direct_dependency_not_subst (inner1 + 1) 0 e2 e1;
+  //   let hBS2' = bigstep_no_dep_no_difference e1' streams1 streams2 row v v' vs2 hBS2 in
+  //   BSLet _ e1 e2 vs2 hBS2'
 
 
+(*
+   We originally had a lemma that said:
+   if expression e mentions variable x, then e[x := e'] mentions e'.
+   we can re-state this as:
+   if expression e mentions variable x, and e' mentions x', then e[x := e'] mentions x'.
+   Do we need it?
+*)
+
+let rec lemma_causal_lift (e: exp 'c 'a) (i: C.index { i <= List.Tot.length 'c }) (t: Type):
+  Lemma (requires (causal e))
+        (ensures (causal (lift1' e i t)))
+        (decreases e) =
+  match e with
+  | XVal _ -> ()
+  | XVar _ -> ()
+  | XBVar _ -> ()
+  | XMu _ e1 ->
+    lemma_causal_lift e1 (i + 1) t;
+    lemma_direct_dependency_lift e1 0 (i + 1) t;
+    ()
+  | _ -> admit ()
 
 
-let bigstep_monotone_inv_next (#outer #inner: nat)
-  (#streams: C.table (outer + 1) inner) (#e: exp { causal e /\ wf e inner }) (#vs: C.vector value outer)
-  (hBS: bigstep (C.table_tl streams) e vs):
-    Tot value =
-  let (| v', hBS' |) = bigstep_monotone_inv' hBS in v'
+let rec lemma_causal_subst (e: exp 'c 'a) (i: C.index { C.has_index 'c i })
+  (p: exp (C.drop1 'c i) (C.get_index 'c i)):
+  Lemma (requires (causal e /\ causal p /\ ~ (direct_dependency e i)))
+        (ensures (causal (subst1' e i p)))
+        (decreases e) =
+  match e with
+  | XVal _ -> ()
+  | XVar _ -> ()
+  | XBVar _ -> ()
+  | XMu _ e1 ->
+    lemma_causal_lift p 0 'a;
+    lemma_causal_subst e1 (i + 1) (lift1 p 'a);
+    lemma_direct_dependency_not_subst 0 (i + 1) e1 (lift1 p 'a);
+    ()
+  | _ -> admit ()
 
-let bigstep_monotone_inv (#outer #inner: nat)
-  (#streams: C.table (outer + 1) inner) (#e: exp { causal e /\ wf e inner }) (#vs: C.vector value outer)
-  (hBS: bigstep (C.table_tl streams) e vs):
-    Tot (bigstep streams e (bigstep_monotone_inv_next hBS :: vs)) =
-  let (| v', hBS' |) = bigstep_monotone_inv' hBS in hBS'
+(* used by ?? *)
+let lemma_causal_subst__causal_XMu {| Pipit.Inhabited.inhabited 'a |}
+  (e: exp ('a :: 'c) 'a):
+  Lemma (requires causal (XMu e))
+        (ensures causal (subst1' e 0 (XMu e))) =
+  lemma_causal_subst e 0 (XMu e)
 
+let rec lemma_bigstep_substitute_elim
+  (i: C.index { i < List.Tot.length 'c })
+  (rows: list (C.row (C.drop1 'c i)) { Cons? rows })
+  (e: exp (C.drop1 'c i) (C.get_index 'c i))
+  (vs: list (C.get_index 'c i) { List.Tot.length rows == List.Tot.length vs })
+  (e': exp 'c 'a)
+  (v': 'a)
+  (hBSse: bigsteps rows e vs)
+  (hBSe': bigstep rows (subst1' e' i e) v'):
+    Tot (bigstep (C.row_zip2_lift1_dropped i rows vs) e' v') (decreases hBSe') =
+  let latest = List.Tot.hd rows in
+  let rows' = C.row_zip2_lift1_dropped i rows vs in
+  let latest' = List.Tot.hd rows' in
+  match e' with
+  | XVal v -> BSVal _ _
+  | XVar _ -> false_elim ()
+  | XBVar i' ->
+    if i = i'
+    then
+      (match hBSse with
+       | BSsS r e_ _ _ v hBSsep hBSe ->
+         bigstep_deterministic hBSe hBSe';
+         assert (v == v');
+         assert (v == List.Tot.hd vs);
+        // TODO row_index lemmas
+         assume (C.row_index 'c latest' i == v);
+         BSVar latest' (List.Tot.tl rows') i)
+    // else if i < i'
+    else
+      (match hBSe' with
+       | BSVar latest prefix ix ->
+         assert (ix == C.index_drop i' i 1);
+         assert (C.row_index (C.drop1 'c i) latest ix == v');
+         assert (C.get_index 'c i' == 'a);
+         // TODO row_index lemmas
+         assume (C.row_index 'c latest' i' == v');
+         BSVar latest' (List.Tot.tl rows') i')
+  | XMu _ e1 ->
+    (match hBSe' with
+    | BSMu _ _ e1' _ hBSe1 ->
+      C.lemma_dropCons 'a 'c (i + 1);
+      assume (C.get_index ('a :: 'c) (i + 1) == C.get_index 'c i);
+      assume (C.drop1 ('a :: 'c) (i + 1) == 'a :: C.drop1 'c i);
+      let lifted: exp (C.drop1 ('a :: 'c) (i + 1)) (C.get_index ('a :: 'c) (i + 1)) = lift1 e 'a in
+      assert (e1' == subst1' e1 (i + 1) lifted);
+      let se: exp ('a :: C.drop1 'c i) 'a = e1' in
+      let se: exp (C.drop1 'c i) 'a = subst1 e1' (XMu e1') in
+      lemma_subst_subst_distribute_XMu e1 i e;
+      assert (subst1 (subst1' e1 (i + 1) lifted) (XMu e1') == subst1' (subst1 e1 (XMu e1)) i e);
+      let hBSe1': bigstep rows se v' = hBSe1 in
+      let hBSX = lemma_bigstep_substitute_elim i rows e vs (subst1 e1 (XMu e1)) v' hBSse hBSe1' in
+      BSMu _ _ e1 _ hBSX
+      // let hBSe1': bigstep rows' (subst1 e1' (subst1' (XMu e1) i e)) v' = hBSe1 in
+      // let hBSe1' = lemma_bigstep_substitute_elim i rows vs _ _ hBSse hBSe1 in
+      // admit ()
+    )
+  | _ -> admit ()
+
+// let rec lemma_bigsteps_substitute_elim
+//   (i: C.index { i < List.Tot.length 'c })
+//   (rows: list (C.row (C.drop1 'c i)))
+//   (e: exp (C.drop1 'c i) (C.get_index 'c i))
+//   (vs: list (C.get_index 'c i) { List.Tot.length rows == List.Tot.length vs })
+//   (e': exp 'c 'a)
+//   (vs': list 'a { List.Tot.length rows == List.Tot.length vs' })
+//   (hBSse: bigsteps rows e vs)
+//   (hBSse': bigsteps rows (subst1' e' i e) vs'):
+//     Tot (bigsteps (C.row_zip2_lift1_dropped i rows vs) e' vs') (decreases hBSse') =
+//   match hBSse with
+//   | BSs0 _ -> BSs0 e'
+//   | BSsS rowsP _ vsP  row v  hBSseP  hBSe ->
+//   match hBSse' with
+//   | BSsS _     _ vs'P _   v' hBSse'P hBSe' ->
+//     let hBSe'' = lemma_bigstep_substitute_elim i rows e vs e' v' hBSse hBSe' in
+//     let rest = lemma_bigsteps_substitute_elim i rowsP e vsP e' vs'P hBSseP hBSse'P in
+//     BSsS (C.row_zip2_lift1_dropped i rowsP vsP) _ vs'P (C.row_lift1_dropped i row v) v' rest hBSe''
+
+let rec lemma_bigstep_substitute_intros_no_dep
+  (i: C.index { i < List.Tot.length 'c })
+  (rows: list (C.row (C.drop1 'c i)))
+  (e: exp (C.drop1 'c i) (C.get_index 'c i))
+  (vs: list (C.get_index 'c i) { List.Tot.length rows == List.Tot.length vs })
+  (e': exp 'c 'a { ~ (direct_dependency e' i) })
+  (r: C.row (C.drop1 'c i))
+  (v: C.get_index 'c i)
+  (a: 'a)
+  (hBSse: bigsteps rows e vs)
+  (hBSe': bigstep (C.row_lift1_dropped i r v :: C.row_zip2_lift1_dropped i rows vs) e' a):
+    Tot (bigstep (r :: rows) (subst1' e' i e) a) (decreases hBSe') =
+  match e' with
+  | XVal _ -> BSVal _ _
+  | XVar _ -> false_elim ()
+  | XBVar i' ->
+    assert (i <> i');
+    admit ()
+  | XFby v0 e1 ->
+    (match rows with
+    | [] -> BSFby1 [r] v0 (subst1' e1 i e)
+    | _ -> admit ()) // BSFbyS r rows v0 _ (subst1' e1 i e))
+  | XMu _ e1 ->
+    (match hBSe' with
+    | BSMu inhabited _ _ _ hBSe1 ->
+      lemma_direct_dependency_not_subst' i 0 e1 (XMu e1);
+      assume (C.get_index ('a :: 'c) (i + 1) == C.get_index 'c i);
+      assume (C.drop1 ('a :: 'c) (i + 1) == 'a :: C.drop1 'c i);
+      let hBSX = lemma_bigstep_substitute_intros_no_dep i rows e vs (subst1 e1 (XMu e1)) r v a hBSse hBSe1 in
+      lemma_subst_subst_distribute_XMu e1 i e;
+      // let lifted: exp (C.drop1 ('a :: 'c) (i + 1)) (C.get_index ('a :: 'c) (i + 1)) = lift1 e 'a in
+      // assert (subst1 (subst1' e1 (i + 1) lifted) (XMu e1') == subst1' (subst1 e1 (XMu e1)) i e);
+      BSMu inhabited _ (subst1' e1 (i + 1) (lift1 e 'a)) _ hBSX)
+  | _ -> admit ()
+
+// let rec lemma_bigsteps_inverts_BSMu
+//   {| Pipit.Inhabited.inhabited 'a |}
+//   (rows: list (C.row 'c))
+//   (e: exp ('a :: 'c) 'a)
+//   (vs: list 'a { List.Tot.length rows == List.Tot.length vs })
+//   (hBSs: bigsteps rows (XMu e) vs):
+//          bigsteps rows (subst1 e (XMu e)) vs =
+//   match hBSs with
+//   | BSs0 _ -> BSs0 (subst1 e (XMu e))
+//   | BSsS rows _ vs row v hBSs' hBS ->
+//     let BSMu _ _ _ e1 hBS' = hBS in
+//     let hBSs'' = lemma_bigsteps_inverts_BSMu rows e vs hBSs' in
+//     BSsS rows _ vs row v hBSs'' hBS'
+
+
+let lemma_bigstep_substitute_elim_XMu
+  {| Pipit.Inhabited.inhabited 'a |}
+  (rows: list (C.row 'c) { Cons? rows })
+  (e: exp ('a :: 'c) 'a { causal (XMu e) })
+  (vs: list 'a { List.Tot.length rows == List.Tot.length vs })
+  (hBSs: bigsteps rows (XMu e) vs):
+    (bigstep (C.row_zip2_cons vs rows) e (List.Tot.hd vs)) =
+    match hBSs with
+    | BSsS _ _ _ _ _ _ hBS ->
+      match hBS with
+      | BSMu _ _ _ _ hBS' ->
+        assume (C.row_zip2_cons vs rows == C.row_zip2_lift1_dropped 0 rows vs);
+        lemma_bigstep_substitute_elim 0 rows (XMu e) vs e (List.Tot.hd vs) hBSs hBS'
+
+let lemma_bigstep_substitute_intros_XMu
+  {| Pipit.Inhabited.inhabited 'a |}
+  (rows: list (C.row 'c))
+  (e: exp ('a :: 'c) 'a { causal (XMu e) })
+  (vs: list 'a { List.Tot.length rows == List.Tot.length vs })
+  (row: C.row 'c)
+  (v v': 'a)
+  (hBSs: bigsteps rows (XMu e) vs)
+  (hBS1: bigstep (C.row_cons v' row :: C.row_zip2_cons vs rows) e v):
+    (bigstep (row :: rows) (XMu e) v) =
+    // let hBSs': bigsteps rows (subst1 e (XMu e)) vs = lemma_bigsteps_inverts_BSMu rows e vs hBSs in
+    // TODO context lemma
+    assume (C.row_zip2_cons vs rows == C.row_zip2_lift1_dropped 0 rows vs);
+    // let hBSs'': bigsteps (C.row_zip2_cons vs rows) e vs = lemma_bigsteps_substitute_elim 0 rows (XMu e) vs e vs hBSs hBSs' in
+    let hBS'': bigstep (row :: rows) (subst1 e (XMu e)) v = lemma_bigstep_substitute_intros_no_dep 0 rows (XMu e) vs e row v' v hBSs hBS1 in
+    BSMu _ (row :: rows) e v hBS''
+
+let rec lemma_bigstep_total
+  (rows: list (C.row 'c) { Cons? rows }) (e: exp 'c 'a { causal e }):
+    Tot (v: 'a & bigstep rows e v) (decreases %[e; rows; 0]) =
+  let hd = List.Tot.hd rows in
+  let tl = List.Tot.tl rows in
+  match e with
+  | XVal v -> (| v, BSVal _ v |)
+  | XVar _ -> false_elim ()
+  | XBVar i ->
+    (| C.row_index 'c hd i, BSVar hd tl i |)
+  | XApp f_e a_e ->
+    assert_norm (causal (XApp f_e a_e) == (causal f_e && causal a_e));
+    let (| f_v, hBSf |) = lemma_bigstep_total rows f_e in
+    let (| a_v, hBSa |) = lemma_bigstep_total rows a_e in
+    (| f_v a_v, BSApp _ _ _ _ _ hBSf hBSa |)
+  | XFby v0 e1 ->
+    (match rows with
+    | [_] -> (| v0, BSFby1 rows v0 e1 |)
+    | latest :: prefix ->
+      let (| v', hBSe1 |) = lemma_bigstep_total prefix e1 in
+      (| v', BSFbyS latest prefix v0 v' e1 hBSe1 |))
+
+  | XMu _ e1 ->
+    let (| vs, hBSs |) = lemma_bigsteps_total tl e in
+    let v' = Pipit.Inhabited.get_inhabited in
+    let (| v, hBS0 |) = lemma_bigstep_total (C.row_cons v' hd :: C.row_zip2_cons vs tl) e1 in
+    let hBS' = lemma_bigstep_substitute_intros_XMu tl e1 vs hd v v' hBSs hBS0 in
+    (| v, hBS' |)
+
+  | _ -> admit ()
+and lemma_bigsteps_total
+  (rows: list (C.row 'c)) (e: exp 'c 'a { causal e }):
+    Tot (vs: list 'a { List.Tot.length vs == List.Tot.length rows } & bigsteps rows e vs) (decreases %[e; rows; 1]) =
+  match rows with
+  | [] -> (| [], BSs0 e |)
+  | r :: rows' ->
+    let (| vs, hBSs |) = lemma_bigsteps_total rows' e in
+    let (| v,  hBS1 |) = lemma_bigstep_total  rows  e in
+    (| v :: vs, BSsS _ _ _ r v hBSs hBS1 |)
